src/PlutusIR/Semantics/Static/normaliser_STLC/gu_naive/SN_STLC_named2.v
@@ -14,45 +14,23 @@ Set Implicit Arguments.
 Unset Strict Implicit.
 Unset Printing Implicit Defensive.
 From PlutusCert Require Import STLC_named STLC_named_typing ARS.
-From PlutusCert Require Import alpha alpha_rename rename util alpha_ctx_sub freshness alpha_freshness step.
-From PlutusCert Require Import SN_STLC_named_naive pre constructions.
+From PlutusCert Require Import alpha.alpha alpha_rename rename util alpha_ctx_sub freshness alpha_freshness.
+From PlutusCert Require Import SN_STLC_named_naive gu_naive.pre gu_naive.constructions.
 
 (* Define an infix operator for bind *)
 Infix ">>=" := bind (at level 50, left associativity).
 
-  (** Normal types *)
-Inductive normal_Ty : term -> Prop :=
-  | NO_TyLam : forall x K T,
-      normal_Ty T ->
-      normal_Ty (tmlam x K T)
-  | NO_neutral : forall T,
-      neutral_Ty T ->
-      normal_Ty T
 
-with neutral_Ty : term -> Prop :=
-  | NE_TyVar : forall X,
-      neutral_Ty (tmvar X)
-  | NE_TyApp : forall T1 T2,
-      neutral_Ty T1 ->
-      normal_Ty T2 ->
-      neutral_Ty (tmapp T1 T2).
 
-(* induction principle for mutual induction*)
-Scheme normal_Ty_mut := Induction for normal_Ty Sort Prop
-with neutral_Ty_mut := Induction for neutral_Ty Sort Prop.
-
-Inductive step_d : term -> term -> Set :=
-| step_beta_d (x : string) (A : type) (s t : term) :
-    normal_Ty s ->
-    normal_Ty t ->
-    step_d (tmapp (tmlam x A s) t) (substituteTCA x t s) (* capture avoiding conservative substitutions *)
-| step_appL_d s1 s2 t :
-    step_d s1 s2 -> step_d (tmapp s1 t) (tmapp s2 t)
-| step_appR_d s t1 t2 :
-    normal_Ty s ->
-    step_d t1 t2 -> step_d (tmapp s t1) (tmapp s t2)
-| step_abs_d x A s1 s2 :
-    step_d s1 s2 -> step_d (tmlam x A s1) (tmlam x A s2).
+Inductive step_nd : term -> term -> Set :=
+| step_beta_nd (x : string) (A : PlutusIR.kind) (s t : term) :
+    step_nd (@tmapp App (@tmlam Lam x A s) t) (substituteTCA x t s) (* capture avoiding conservative substitutions *)
+| step_appL_nd B s1 s2 t :
+    step_nd s1 s2 -> step_nd (@tmapp B s1 t) (@tmapp B s2 t)
+| step_appR_nd B s t1 t2 :
+    step_nd t1 t2 -> step_nd (@tmapp B s t1) (@tmapp B s t2)
+| step_abs_nd B x A s1 s2 :
+    step_nd s1 s2 -> step_nd (@tmlam B x A s1) (@tmlam B x A s2).
 
 Lemma in_ftv_existsb_true t s :
   In s (ftv t) -> existsb (eqb s) (ftv t) = true.
@@ -112,12 +90,13 @@ induction s; simpl.
 - autorewrite with substituteTCA. f_equal.
   + eapply IHs1; eapply nc_app_l. eauto.
   + eapply IHs2; eapply nc_app_r. eauto.
+- autorewrite with substituteTCA. auto.
 Qed.
 
 (* If t has globally unique binders (and free variables to make it easier)
     then deterministic step and naive step coincide*)
 Lemma GU_step_d_implies_step_na t t' : 
-    GU t -> step_d t t' -> step_naive t t'.
+    GU t -> step_nd t t' -> step_naive t t'.
 Proof.
     intros HGU_vars H.
     induction H.
@@ -161,6 +140,7 @@ Proof.
   - constructor.
     + eapply IHs'1; eauto. eapply not_ftv_app_not_left; eauto.
     + eapply IHs'2; eauto. eapply not_ftv_app_not_right; eauto.
+  - constructor.
 Qed.
 
 Lemma subs_preserves_alpha' X T i : forall s s' R1 R2 R,
@@ -171,11 +151,11 @@ Lemma subs_preserves_alpha' X T i : forall s s' R1 R2 R,
   R2 ⊢ i ~ s' ->
   R ⊢ substituteTCA X T s ~ substituteTCA X T s'.
 Proof.
-  induction i as [xi | xi ? bi | i1 IHi1 i2 IHi2];
+  induction i as [xi | B xi ? bi | B i1 IHi1 i2 IHi2|d];
   intros s s' R1 R2 R Ha_X Ha_T Htrans Hαs Hαs';
-  inversion Hαs as [xs ? ? Hαvs | xs ? ? bs ? ? Hαbs | s1 ? s2 ? ? Hαs1 Hαs2 ]; subst;
-  inversion Hαs' as [? xs' ? Hαvs' |? xs' ? ? bs' ? Hαbs' | ? s1' ? s2' ? Hαs1' Hαs2']; subst;
-  autorewrite with capms; simpl.
+    inversion Hαs as [xs ? ? Hαvs | xs ? ? bs ? ? Hαbs | s1 ? s2 ? ? Hαs1 Hαs2 |]; subst;
+    inversion Hαs' as [? xs' ? Hαvs' |? xs' ? ? bs' ? Hαbs' | ? s1' ? s2' ? Hαs1' Hαs2'|]; 
+    subst; simpl.
   - (* Case: tmvar *)
     repeat rewrite substituteTCA_equation_1.
     assert (Hαv: AlphaVar R xs xs'). { eapply alpha_var_trans; eauto. }
@@ -195,37 +175,37 @@ Proof.
     (* remember (fresh2 _ bs) as b; rewrite cons_to_append in Heqb.
     remember (fresh2 _ bs') as b'; rewrite cons_to_append in Heqb'. *)
     (* idk, but it is true.*)
-    destr_eqb_eq xs X.
+    destr_eqb_eq x X.
     + rewrite substituteTCA_equation_2.
-      remember (fresh2 _ bs) as b; rewrite cons_to_append in Heqb.
+      remember (fresh2 _ s1) as b; rewrite cons_to_append in Heqb.
       rewrite String.eqb_refl.
       eapply @alpha_sym with (ren := sym_alpha_ctx R); eauto with α_eq_db.
       eapply substituteTCA_vacuous; eauto with α_eq_db.
-      eapply @alpha_preserves_no_ftv with (x := X) (s := tmlam X t bs).
+      eapply @alpha_preserves_no_ftv with (x := X) (s := tmlam X k s1).
       * apply ftv_lam_no_binder.
       * eauto with α_eq_db.
       * inversion Ha_X; eauto.
-    + destr_eqb_eq xs' X.
-      * assert (substituteTCA X T (tmlam X t bs') = tmlam X t bs').
+    + destr_eqb_eq y X.
+      * assert (Hvac_sub: substituteTCA X T (@tmlam B X k s2) = @tmlam B X k s2).
         {
           rewrite substituteTCA_equation_2.
           rewrite String.eqb_refl.
           reflexivity.
         }
-        rewrite H0.
+        rewrite Hvac_sub.
         eapply substituteTCA_vacuous; eauto with α_eq_db.
-        eapply @alpha_preserves_no_ftv with (x := X) (s := tmlam X t bs').
+        eapply @alpha_preserves_no_ftv with (x := X) (s := tmlam X k s2).
         -- apply ftv_lam_no_binder.
         -- eauto with α_eq_db.
         -- inversion Ha_X; eauto. eapply @alphavar_sym with (ren := R); eauto with α_eq_db.
       * autorewrite with substituteTCA.
-        rewrite <- String.eqb_neq in H. rewrite String.eqb_sym in H. rewrite H.
-        rewrite <- String.eqb_neq in H0. rewrite String.eqb_sym in H0. rewrite H0.
+        rewrite <- String.eqb_neq in H1. rewrite String.eqb_sym in H1. rewrite H1.
+        rewrite <- String.eqb_neq in H2. rewrite String.eqb_sym in H2. rewrite H2.
 
-        destruct (existsb (eqb xs) (ftv T)) eqn:Hin; destruct (existsb (eqb xs') (ftv T)) eqn:Hin'.
+        destruct (existsb (eqb x) (ftv T)) eqn:Hin; destruct (existsb (eqb y) (ftv T)) eqn:Hin'.
         -- simpl.
-           remember (fresh2 _ bs) as Y'.
-           remember (fresh2 _ bs') as Y''.
+           remember (fresh2 _ s1) as Y'.
+           remember (fresh2 _ s2) as Y''.
            constructor.
            eapply IHbi; eauto.
            ++ eapply alpha_extend_fresh; auto.
@@ -246,7 +226,7 @@ Proof.
            ++ eapply alpha_trans_rename_left; eauto.
            ++ eapply alpha_trans_rename_right; eauto.
         -- simpl.
-           remember (fresh2 _ bs) as Y'.
+           remember (fresh2 _ s1) as Y'.
            constructor.
             eapply IHbi; eauto.
             ++ eapply alpha_extend_fresh; auto.
@@ -254,7 +234,7 @@ Proof.
                  intros Hcontra. apply ftv_var in Hcontra.  subst. contradiction.
                  apply in_cons. apply in_eq.
               ** intros Hcontra. apply ftv_var in Hcontra. subst.
-                 rewrite String.eqb_neq in H0. contradiction.
+                 rewrite String.eqb_neq in H2. contradiction.
             ++ eapply alpha_extend_fresh; auto.
               ** eapply fresh2_over_tv_value_sigma with (X := X) (s := T) in HeqY'.
                  intros Hcontra. apply extend_ftv_to_tv in Hcontra. contradiction.
@@ -263,12 +243,12 @@ Proof.
             ++ eauto with α_eq_db.
             ++ eapply alpha_trans_rename_left; eauto.
         -- simpl.
-           remember (fresh2 _ _) as Y'.
+           remember (fresh2 _ s2) as Y'.
            constructor.
            eapply IHbi; eauto. 
            ++ eapply alpha_extend_fresh; auto.
               ** intros Hcontra. apply ftv_var in Hcontra; subst.
-                  rewrite String.eqb_neq in H. contradiction.
+                  rewrite String.eqb_neq in H1. contradiction.
               **  
                 eapply fresh2_over_key_sigma with (X := X) in HeqY'.
                  intros Hcontra. apply ftv_var in Hcontra.  subst. contradiction.
@@ -284,9 +264,9 @@ Proof.
         -- constructor; eapply IHbi; eauto.
            ++ apply alpha_extend_fresh; auto.
               ** intros Hcontra. apply ftv_var in Hcontra; subst.
-                  rewrite String.eqb_neq in H. contradiction.
+                  rewrite String.eqb_neq in H1. contradiction.
               ** intros Hcontra. apply ftv_var in Hcontra; subst.
-                  rewrite String.eqb_neq in H0. contradiction.
+                  rewrite String.eqb_neq in H2. contradiction.
            ++ eapply alpha_extend_fresh; auto.
               eapply not_in_ftv_existsb_false. auto.
               eapply not_in_ftv_existsb_false. auto.
@@ -295,6 +275,8 @@ Proof.
     constructor.
     + eapply IHi1; eauto.
     + eapply IHi2; eauto.
+  - autorewrite with substituteTCA.
+    constructor.
 Qed.
 
 Lemma substituteTCA_preserves_alpha s s' ren X U:
@@ -326,49 +308,20 @@ Proof.
   - apply to_GU'__NC.
 Qed.
 
-Lemma alpha_preserves_normal_Ty__neutral_Ty s s' R :
-  R ⊢ s ~ s' -> ((normal_Ty s -> normal_Ty s') * (neutral_Ty s -> neutral_Ty s')).
-Proof.
-  intros Ha_s.
-  generalize dependent R.
-  generalize dependent s'.
-  induction s; intros s' R Ha_s; inversion Ha_s; subst.
-  - split; repeat constructor.
-  - edestruct IHs; eauto.
-    split.
-    + intros. constructor. eapply n. inversion H; subst. auto. inversion H0.
-    + intros. inversion H.
-  - edestruct IHs1; eauto.
-    edestruct IHs2; eauto.
-    split.
-    + intros. constructor. constructor.
-      * eapply n0. inversion H. inversion H0; subst. auto.
-      * inversion H; subst. inversion H0. auto.
-    + intros. inversion H; subst. constructor; eauto.
-Qed.
-
-Lemma alpha_preserves_normal_Ty s s' R :
-  R ⊢ s ~ s' -> normal_Ty s -> normal_Ty s'.
-Proof.
-  intros Ha_s Hn.
-  edestruct (alpha_preserves_normal_Ty__neutral_Ty Ha_s) as [H _].
-  auto.
-Qed.
-
 (* Main lemma for going from using t alpha t' in SN t' to SN t*)
-Lemma step_d_preserves_alpha ren s t s' :
-  Alpha ren s t -> step_d s s' -> {t' & (step_d t t') * (Alpha ren s' t')}%type.
+Lemma step_nd_preserves_alpha ren s t s' :
+  Alpha ren s t -> step_nd s s' -> {t' & (step_nd t t') * (Alpha ren s' t')}%type.
 Proof.
   intros Halpha Hstep.
   generalize dependent t.
   generalize dependent ren.
   induction Hstep; intros ren t0 Halpha; inversion Halpha; subst.
-  - inversion H2; subst.
+  - inversion H4; subst.
     remember (alpha_capms_to_naive x t s).
     destruct s1 as [s' [ [Halpha1 Halpha2] Halpha3] ].
     eexists.
     split.
-    + apply step_beta_d; eapply alpha_preserves_normal_Ty; eauto.
+    + apply step_beta_nd.
     + eapply @alpha_trans with (t := sub x t s').
       * apply id_left_trans.
       * change (ctx_id_left ren) with (nil ++ ctx_id_left ren).
@@ -396,24 +349,22 @@ Proof.
            apply alpha_extend_ids_right.
            ++ apply ctx_id_right_is_id.
            ++ eapply alpha_sym. constructor. eauto.
-  - destruct (IHHstep ren s3 H2) as [t1_α [Hstep' Halpha'] ].
-    exists (tmapp t1_α t2); split.
-    + apply step_appL_d. assumption.
+  - destruct (IHHstep ren s3 H4) as [t1_α [Hstep' Halpha'] ].
+    exists (@tmapp B t1_α t2); split.
+    + apply step_appL_nd. assumption.
     + apply alpha_app; assumption.
-  - destruct (IHHstep ren t4 H4) as [tα [Hstep' Halpha'] ].
-    exists (tmapp s2 tα); split.
-    + apply step_appR_d.
-      * eapply alpha_preserves_normal_Ty; eauto.
-      * assumption.
+  - destruct (IHHstep ren t4 H5) as [tα [Hstep' Halpha'] ].
+    exists (@tmapp B s2 tα); split.
+    + apply step_appR_nd; auto.
     + apply alpha_app; assumption.
-  - destruct (IHHstep ((x, y)::ren) s3 H4) as [tα [Hstep' Halpha'] ].
-    exists (tmlam y A tα); split.
-    + apply step_abs_d. assumption.
+  - destruct (IHHstep ((x, y)::ren) s3 H5) as [tα [Hstep' Halpha'] ].
+    exists (@tmlam B y A tα); split.
+    + apply step_abs_nd. assumption.
     + apply alpha_lam; assumption.    
 Qed.
 
-Lemma step_d_implies_step_gu_na t t' : 
-    step_d t t' ->  
+Lemma step_nd_implies_step_gu_na t t' : 
+    step_nd t t' ->  
     {t_α & step_gu_naive t t_α * (nil ⊢ t' ~ t_α)}%type.
 Proof.
     remember (to_GU t) as t_GU.
@@ -428,7 +379,7 @@ Proof.
       apply to_GU__GU.
     }
     intros.
-    remember (step_d_preserves_alpha H_alpha H) as Hstep_GU.
+    remember (step_nd_preserves_alpha H_alpha H) as Hstep_GU.
     destruct Hstep_GU as [t_GU' [Hstep_GU Halpha_GU] ].
     exists t_GU'.
     split; auto.
@@ -438,17 +389,17 @@ Proof.
     + subst. auto.
 Qed.
 
-Theorem α_preserves_sn_d s s' :
-  Alpha [] s s' -> (@sn term step_d) s -> (@sn term step_d) s'.
+Theorem α_preserves_sn_nd s s' :
+  Alpha [] s s' -> (@sn term step_nd) s -> (@sn term step_nd) s'.
 Proof.
   intros Hα Hsn.
   generalize dependent s'.
   induction Hsn. intros s' Hα.
   apply SNI.
   intros y1 Hstep.
-  assert ({y1_α & prod (step_d x y1_α) (nil ⊢ y1 ~ y1_α)}) as [y1_α [Hstep' Hα'] ].
+  assert ({y1_α & prod (step_nd x y1_α) (nil ⊢ y1 ~ y1_α)}) as [y1_α [Hstep' Hα'] ].
   {
-    eapply step_d_preserves_alpha; auto.
+    eapply step_nd_preserves_alpha; auto.
     - eapply alpha_sym in Hα. exact Hα. apply alpha_sym_nil.
     - assumption.
   }
@@ -457,7 +408,7 @@ Proof.
   - eapply alpha_sym. apply alpha_sym_nil. exact Hα'.
 Qed.
 
-Lemma SN_na_to_SN_d t : (@sn term step_gu_naive) t -> (@sn term step_d) t.
+Lemma SN_na_to_SN_nd t : (@sn term step_gu_naive) t -> (@sn term step_nd) t.
 Proof.
   intros Hsn_nd.
   apply SNI.
@@ -466,21 +417,21 @@ Proof.
   induction Hsn_nd; intros t Hstep_d.
   assert (Hstep_alpha: {t' & prod (step_gu_naive x t') (Alpha nil t t')}).
   {
-    eapply step_d_implies_step_gu_na; eauto.
+    eapply step_nd_implies_step_gu_na; eauto.
   }
   destruct Hstep_alpha as [t' [Hstep Halpha] ].
   specialize (X t' Hstep).
-  apply α_preserves_sn_d with t'.
+  apply α_preserves_sn_nd with t'.
   - eapply alpha_sym; [apply alpha_sym_nil |].
     assumption.
   - apply SNI. 
     exact X.
 Qed.
 
-Theorem strong_normalization E s T : has_type E s T -> (@sn term step_d) s.
+Theorem strong_normalization E s T : STLC_named_typing.has_kind E s T -> (@sn term step_nd) s.
   intros.
   apply SN_naive in H. 
-  apply SN_na_to_SN_d.
+  apply SN_na_to_SN_nd.
   assumption.
 Qed.
 
