src/PlutusIR/Semantics/Static/normaliser_STLC/gu_naive/port_plut2.v
@@ -12,202 +12,86 @@ Require Import Coq.Arith.PeanoNat.
 Import ListNotations.
 Require Import Ascii.
 
-From PlutusCert Require Import port_plut util Util.List. (* I don't understand why we need this for ftv defintion*)
+From PlutusCert Require Import SN_STLC_named_naive SN_STLC_named2 util Util.List STLC_named STLC_named_typing plutus_kinding_set. (* I don't understand why we need this for ftv defintion*)
+From PlutusCert Require PlutusIR Static.TypeSubstitution Normalisation.Type_reduction.
 
-Inductive BType := L | F. (* Lam or Forall*)
-
-(** Types *)
-Inductive term :=
-  | tmvar : string -> term
-  | tmlam : BType -> string -> type -> term -> term
-  | tmapp : term -> term -> term
-.
-
-(** Substitutions *)
-Function ftv (T : term) : list string :=
-    match T with
-    | tmvar X =>
-        [X]
-    | tmlam B X K1 T' =>
-        remove string_dec X (ftv T')
-    | tmapp T1 T2 =>
-        ftv T1 ++ ftv T2
-    end.
-
-Fixpoint btv (T : term) : list string :=
-    match T with
-    | tmvar X =>
-        []
-    | tmlam B X K1 T' =>
-      X :: btv T'
-    | tmapp T1 T2 =>
-        btv T1 ++ btv T2
-    end.
-
-(* Bound and free type variables *)
-Fixpoint tv (s : term) : list string :=
-  match s with
-  | tmvar x => x::nil
-  | tmlam B x A s => x :: tv s
-  | tmapp s t => tv s ++ tv t
-  end.
-
-(** * Capture-avoiding substitution of types *)
-
-Fixpoint tv_keys_env (sigma : list (string * term)) : list string :=
-  match sigma with
-  | nil => nil
-  | (x, t)::sigma' => x :: (tv t) ++ (tv_keys_env sigma')
-  end.
-
-Definition fresh2 (sigma : list (string * term)) (T : term) : string :=
-  "a" (* new*)
-  ++ String.concat EmptyString (
-    tv_keys_env sigma ++ tv T
-  ).
-
-Definition fresh (X : string) (U T : term) : string :=
-  "a" ++ X ++ (String.concat EmptyString (ftv U)) ++ (String.concat EmptyString (ftv T)).
-
-Lemma fresh__X : forall X U T,
-    X <> fresh X U T.
-Proof with eauto.
-  intros. intros Hcon.
-  induction X; induction (ftv U); induction (ftv T).
-  all: simpl in Hcon.
-  all: inversion Hcon; subst...
-Qed.
-
-Lemma fresh__S : forall X U T,
-    ~ In (fresh X U T) (ftv U).
-Proof. Abort.
-
-Lemma fresh__T : forall X U T,
-    ~ In (fresh X U T) (ftv T).
-Proof. Abort.
-
-Fixpoint rename (X Y : string) (T : term) :=
-  match T with
-  | tmvar Z =>
-      if X =? Z then tmvar Y else tmvar Z
-  | tmlam B Z K T0 =>
-      if X =? Z then tmlam B Z K T0
-      else tmlam B Z K (rename X Y T0)
-  | tmapp T1 T2 =>
-      tmapp (rename X Y T1) (rename X Y T2)
-  end.
-
-(* Size of a term *)
-
-Fixpoint size (T : term) : nat :=
-  match T with
-  | tmvar Y => 1
-  | tmlam B bX K T0 => 1 + size T0
-  | tmapp T1 T2 => 1 + size T1 + size T2
-  end.
-
-
-Lemma rename_preserves_size : forall T X Y,
-    size T = size (rename X Y T).
-Proof.
-  unfold rename.
-  induction T; intros; simpl; eauto.
-  - destruct (X =? s); eauto.
-  - destruct (X =? s); simpl; eauto.
-Qed.
-
-Equations? substituteTCA (X : string) (U T : term) : term by wf (size T) :=
-  substituteTCA X U (tmvar Y) =>
-      if X =? Y then U else tmvar Y ;
-  substituteTCA X U (@tmlam B Y K T) =>
-      if X =? Y
-        then
-          @tmlam B Y K T
-        else
-          if existsb (String.eqb Y) (ftv U)
-            then
-              let Y' := fresh2 ((Y, tmvar Y)::(X, U)::nil) T in
-              let T' := rename Y Y' T in
-              @tmlam B Y' K (substituteTCA X U T')
-            else
-              @tmlam B Y K (substituteTCA X U T) ;
-  substituteTCA X U (tmapp T1 T2) =>
-      tmapp (substituteTCA X U T1) (substituteTCA X U T2)
-  .
-Proof.
-  all: try solve
-    [ lia
-    || replace T' with (rename Y Y' T); eauto; rewrite <- rename_preserves_size; eauto
-    ].
-Qed.
-
-
-Inductive step_nd : term -> term -> Type :=
-| step_beta_d (x : string) (A : type) (s t : term) :
-  (* This allows for more steps then should be allowed.
-      e.g. tmapp (forall B x A s) t) will now beta reduce.
-
-      But that is no problem! As long as step_nd allows all steps that step_plut allows.
-  *)
-    step_nd (tmapp (@tmlam L x A s) t) (substituteTCA x t s) (* capture avoiding conservative substitutions *)
-| step_appL_d s1 s2 t :
-    step_nd s1 s2 -> step_nd (tmapp s1 t) (tmapp s2 t)
-| step_appR_d s t1 t2 :
-    step_nd t1 t2 -> step_nd (tmapp s t1) (tmapp s t2)
-| step_abs_d B x A s1 s2 :
-    step_nd s1 s2 -> step_nd (@tmlam B x A s1) (@tmlam B x A s2).
-
-Set Implicit Arguments.
 
 (** Substitutions *)
 
 (* from plut to annotated stlc*)
-Fixpoint f (t : term_plut) : term :=
+Fixpoint f (t : PlutusIR.ty) : term :=
   match t with
-  | plutvar x => tmvar x
-  | plutlam x A t => @tmlam L x A (f t)
-  | plutforall x A t => @tmlam F x A (f t)
-  | plutapp t1 t2 => tmapp (f t1) (f t2)
+  | PlutusIR.Ty_Var x => tmvar x
+  | PlutusIR.Ty_Lam x A t => @tmlam Lam x A (f t)
+  | PlutusIR.Ty_Forall x A t => @tmlam ForAll x A (f t)
+  | PlutusIR.Ty_Fun t1 t2 => @tmapp Fun (f t1) (f t2)
+  | PlutusIR.Ty_App t1 t2 => @tmapp App (f t1) (f t2)
+  | PlutusIR.Ty_IFix f1 t1 => @tmapp IFix (f f1) (f t1)
+  | PlutusIR.Ty_Builtin d => tmbuiltin d
   end.
 
 Require Import Coq.Program.Equality.
 
+Set Printing Implicit.
+
 Lemma f_preserves_rename s fr T :
-  rename s fr (f T) = f (port_plut.rename s fr T).
+  rename s fr (f T) = f (TypeSubstitution.rename s fr T).
 Proof.
   induction T.
   - simpl.
-    destr_eqb_eq s s0.
-    + simpl. auto.
-    + simpl. auto.
-  - simpl.
-    destr_eqb_eq s s0.
-    + simpl. auto.
+    destr_eqb_eq s t.
+    + simpl. auto. unfold TypeSubstitution.rename. simpl. rewrite String.eqb_refl. simpl.
+      unfold rename. simpl. rewrite String.eqb_refl. simpl. auto.
+    + unfold rename. unfold TypeSubstitution.rename. simpl. rewrite <- String.eqb_neq in H. rewrite H. simpl. auto.
+  - simpl. unfold rename. simpl. f_equal. auto. auto.
+  - simpl. unfold rename. simpl. f_equal. auto. auto.
+  - unfold rename. simpl.
+    unfold TypeSubstitution.rename.
+    simpl.
+    destr_eqb_eq s b.
+    + rewrite mren_id.
+      simpl. auto.
     + simpl. f_equal. auto.
-  - simpl.
-    destr_eqb_eq s s0.
-    + simpl. auto.
-    + simpl. f_equal; auto.
-  - simpl.
-    f_equal; auto.
+  - simpl. unfold rename. simpl. auto.
+  - unfold rename. simpl.
+    unfold TypeSubstitution.rename.
+    simpl.
+    destr_eqb_eq s b.
+    + rewrite mren_id.
+      simpl. auto.
+    + simpl. f_equal. auto.
+  - simpl. unfold rename. simpl. f_equal. auto. auto.
 Qed.
 
 Lemma f_preserves_ftv T :
-  ftv (f T) = port_plut.ftv T.
+  ftv (f T) = TypeSubstitution.ftv T.
 Proof.
   induction T; simpl; try f_equal; auto.
 Qed.
+
+(* TODO: This tv definition should be somewhere else! *)
+Fixpoint plutusTv (t : PlutusIR.ty) : list string :=
+  match t with
+  | PlutusIR.Ty_Var x => [x]
+  | PlutusIR.Ty_Lam x A t => x :: (plutusTv t)
+  | PlutusIR.Ty_Forall x A t => x :: (plutusTv t)
+  | PlutusIR.Ty_Fun t1 t2 => plutusTv t1 ++ plutusTv t2
+  | PlutusIR.Ty_App t1 t2 => plutusTv t1 ++ plutusTv t2
+  | PlutusIR.Ty_IFix f1 t1 => plutusTv f1 ++ plutusTv t1
+  | PlutusIR.Ty_Builtin d => []
+  end.
 
 Lemma f_preserves_tv T :
-  tv (f T) = port_plut.tv T.
+  tv (f T) = plutusTv T.
 Proof.
   induction T; simpl; try f_equal; auto.
 Qed.
 
+(* Not true currently*)
 Lemma f_preserves_fresh2 x y s s' T :
-  fresh2 ((x, f s)::(y, f s')::nil) (f T) = port_plut.fresh2 ((x, s)::(y, s')::nil) T.
+  fresh2 ((x, f s)::(y, f s')::nil) (f T) = TypeSubstitution.fresh y s' T.
 Proof.
-  simpl.
+  (* simpl.
   unfold fresh2.
   unfold port_plut.fresh2.
   rewrite f_preserves_tv.
@@ -223,13 +107,13 @@ Proof.
     f_equal.
   }
   rewrite Htv_keys_env.
-  reflexivity.
-Qed.
+  reflexivity. *)
+Admitted.
 
 Require Import Coq.Arith.Wf_nat.
 
 Lemma f_preserves_substituteTCA X U T :
-  (f (port_plut.substituteTCA X U T)) = (substituteTCA X (f U) (f T)).
+  (f (TypeSubstitution.substituteTCA X U T)) = (substituteTCA X (f U) (f T)).
 Proof.
   remember (f T) as fT.
   remember (size fT) as n.
@@ -240,100 +124,131 @@ Proof.
   dependent induction fT; subst.
   + induction T; subst; inversion HeqfT; subst.
     autorewrite with substituteTCA.
-    destr_eqb_eq X s0; auto.
-  + induction T; subst; inversion HeqfT; subst.
-    * autorewrite with substituteTCA.
-      destr_eqb_eq X s0; eauto.
-      rewrite <- (f_preserves_ftv).
-      destruct (existsb (String.eqb s0) (ftv (f U))) eqn:Heq.
-      -- 
-          simpl.
-          remember (fresh2 _ _) as fr.
-          remember (port_plut.fresh2 _ _) as fr'.
-          assert (Hfr_pres: fr' = fr).
-          {
-            subst.
-            symmetry.
-            assert (Hfpluvar: f (plutvar s0) = tmvar s0) by auto.
-            rewrite <- Hfpluvar.
-            rewrite f_preserves_fresh2.
-            reflexivity.
-          }
-          rewrite Hfr_pres.
-          f_equal.
-          ++ eapply H; eauto.
-            ** rewrite <- rename_preserves_size.
-               simpl.
-               lia.
-            ** apply f_preserves_rename.
-      -- simpl.
-          f_equal.
-          eapply H; eauto. simpl. lia.
-
-
-
-      (* TODO: EXACTLY IDENTICAL TO ABOVE*)
-      * autorewrite with substituteTCA.
-      destr_eqb_eq X s0; eauto.
-      rewrite <- (f_preserves_ftv).
-      destruct (existsb (String.eqb s0) (ftv (f U))) eqn:Heq.
-      -- 
-          simpl.
-          remember (fresh2 _ _) as fr.
-          remember (port_plut.fresh2 _ _) as fr'.
-          assert (Hfr_pres: fr' = fr).
-          {
-            subst.
-            symmetry.
-            assert (Hfpluvar: f (plutvar s0) = tmvar s0) by auto.
-            rewrite <- Hfpluvar.
-            rewrite f_preserves_fresh2.
-            reflexivity.
-          }
-          rewrite Hfr_pres.
-          f_equal.
-          ++ eapply H; eauto.
-            ** rewrite <- rename_preserves_size.
-               simpl.
-               lia.
-            ** apply f_preserves_rename.
-      -- simpl.
-          f_equal.
-          eapply H; eauto. simpl. lia.
-
-        (* END TODO*)
-
+    destr_eqb_eq X t; auto.
   + induction T; subst; inversion HeqfT; subst.
     
-    autorewrite with substituteTCA.
-    simpl.
-    f_equal; eauto.
-    * eapply H; auto. simpl. lia.
-    * eapply H; auto. simpl. lia.
-Qed.
+    {
+      autorewrite with substituteTCA.
+      destr_eqb_eq X b; eauto.
+      rewrite <- (f_preserves_ftv).
+      destruct (existsb (String.eqb b) (ftv (f U))) eqn:Heq.
+      -- 
+          simpl.
+          remember (fresh2 _ _) as fr.
+          remember (TypeSubstitution.fresh _ _ _) as fr'.
+          assert (Hfr_pres: fr' = fr).
+          {
+            (* Not currently true, but probably possible to change on both sides*)
+            subst.
+            symmetry.
+            assert (tmvar b = f (PlutusIR.Ty_Var b)).
+            {
+              simpl.
+              auto.
+            }
+            rewrite H1.
+            eapply f_preserves_fresh2.
+          }
+          rewrite Hfr_pres.
+          f_equal.
+          ++ eapply H; eauto.
+            ** rewrite <- rename_preserves_size.
+               simpl.
+               lia.
+            ** apply f_preserves_rename.
+      -- simpl.
+         f_equal.
+          eapply H; eauto. simpl. lia.
+    }
 
+
+(* TODO: EXACTLY IDENTICAL TO ABOVE*)
+
+     {
+      autorewrite with substituteTCA.
+      destr_eqb_eq X b; eauto.
+      rewrite <- (f_preserves_ftv).
+      destruct (existsb (String.eqb b) (ftv (f U))) eqn:Heq.
+      -- 
+          simpl.
+          remember (fresh2 _ _) as fr.
+          remember (TypeSubstitution.fresh _ _ _) as fr'.
+          assert (Hfr_pres: fr' = fr).
+          {
+            (* Not currently true, but probably possible to change on both sides*)
+            subst.
+            symmetry.
+            assert (tmvar b = f (PlutusIR.Ty_Var b)).
+            {
+              simpl.
+              auto.
+            }
+            rewrite H1.
+            eapply f_preserves_fresh2.
+          }
+          rewrite Hfr_pres.
+          f_equal.
+          ++ eapply H; eauto.
+            ** rewrite <- rename_preserves_size.
+               simpl.
+               lia.
+            ** apply f_preserves_rename.
+      -- simpl.
+         f_equal.
+          eapply H; eauto. simpl. lia.
+    }
+         
+    
+  + induction T; subst; inversion HeqfT; subst.
+    all: autorewrite with substituteTCA; simpl; f_equal; eauto; eapply H; auto; simpl; lia. 
+  + assert (T = PlutusIR.Ty_Builtin d).
+    {
+      destruct T; auto; inversion HeqfT. auto.
+    }
+    subst.
+    autorewrite with substituteTCA.
+    simpl. auto.
+Qed.
         
 Theorem f_preserves_step s s' :
-  step_plut s s' -> step_nd (f s) (f s').
+  Type_reduction.step s s' -> step_nd (f s) (f s').
 Proof.
   intros H.
-  induction H; simpl; eauto.
+  induction H; simpl; eauto; try solve [constructor; eauto].
   - rewrite f_preserves_substituteTCA.
     constructor.
-  - constructor. assumption.
-  - constructor. assumption.
-  - constructor. assumption.
-  - constructor. assumption.
 Qed.
 
-Inductive sn {X : Type} {e : X -> X -> Type } x : Type :=
-| SNI : (forall y, e x y -> sn y) -> sn x.
+Set Printing Implicit.
+
+Require Import Coq.Program.Equality.
+
+Theorem f_preserves_kind Δ s K :
+  plutus_kinding_set.has_kind Δ s K -> STLC_named_typing.has_kind Δ (f s) K.
+Proof.
+  intros.
+  induction H; simpl; eauto.
+  - constructor.
+    auto.
+  - constructor.
+    + eauto.
+    + eauto.
+  - eapply STLC_named_typing.K_IFix; eauto.
+  - constructor.
+    auto.
+  - constructor.
+    exact h.
+  - constructor.
+    auto.
+  - eapply STLC_named_typing.K_App; eauto.
+Qed.  
+
 
 (*
 Jacco: Dit is blijkbaar een forward simulation
 *)
-Lemma sn_preimage2 {e2 : term_plut -> term_plut -> Type} {e : term -> term -> Type} (h : term_plut -> term) (x : term_plut) :
-  (forall x y, e2 x y -> e (h x) (h y)) -> @sn term e (h x) -> @sn term_plut e2 x.
+Lemma sn_preimage2 {e2 : PlutusIR.ty -> PlutusIR.ty -> Type} {e : term -> term -> Type} (h : PlutusIR.ty -> term) (x : PlutusIR.ty) :
+  (forall x y, e2 x y -> e (h x) (h y)) -> @sn term e (h x) -> @sn PlutusIR.ty e2 x.
 Proof.
   intros A B.
   remember (h x) as v. (* this allows us to keep B : sn v as an hypothesis*)
@@ -353,24 +268,19 @@ Proof.
   - reflexivity.
 Qed.
 
-(* todo: well kinded assumption.
-  So we need to convert that from the step_plut one.
-  if s is plut_well_kinded, then (f s) is nd_well_kinded
- *)
-Theorem sn_step_nd : forall s, @sn term step_nd s.
-Admitted.
-
-Theorem sn_step_plut : forall s, @sn term step_nd (f s) -> @sn term_plut step_plut s.
+Theorem sn_step_plut : forall s, @sn term step_nd (f s) -> @sn PlutusIR.ty Type_reduction.step s.
 Proof.
   intros s.
-  eapply @sn_preimage2 with (h := f) (e2 := step_plut) (e := step_nd).
+  eapply @sn_preimage2 with (h := f) (e2 := Type_reduction.step) (e := step_nd).
   apply f_preserves_step.
 Qed.
 
-Corollary sn_step_plut2 : forall s, @sn term_plut step_plut s.
+Corollary sn_step_plut2 s Δ K : plutus_kinding_set.has_kind Δ s K -> @sn PlutusIR.ty Type_reduction.step s.
 Proof.
-  intros s.
-  eapply sn_preimage2 with (h := f).
-  apply f_preserves_step.
-  apply sn_step_nd.
+  intros Hwk.
+  eapply sn_preimage2. 
+  - apply f_preserves_step.
+  - eapply strong_normalization with (E := Δ) (T := K).
+    eapply f_preserves_kind.
+    auto.
 Qed.
