src/PlutusIR/Semantics/Static/normaliser_STLC/gu_naive/plutus_kinding_set.v
@@ -1,0 +1,80 @@
+
+Require Import PlutusCert.PlutusIR.
+Require Import PlutusCert.Util.List.
+Require Import Coq.Strings.String.
+Require Import Coq.Lists.List.
+
+Reserved Notation "'|-*_uni' T ':' K" (at level 40, T at level 0, K at level 0).
+Inductive has_kind_uni : DefaultUni -> kind -> Set :=
+  | K_DefaultUniInteger :
+      |-*_uni DefaultUniInteger : Kind_Base
+  | K_DefaultUniByteString :
+      |-*_uni DefaultUniByteString : Kind_Base
+  | K_DefaultUniString :
+      |-*_uni DefaultUniString : Kind_Base
+  | K_DefaultUniUnit :
+      |-*_uni DefaultUniUnit : Kind_Base
+  | K_DefaultUniBool :
+      |-*_uni DefaultUniBool : Kind_Base
+  | K_DefaultUniData :
+      |-*_uni DefaultUniData : Kind_Base
+  | K_DefaultUniBLS12_381_G1_Element :
+      |-*_uni DefaultUniBLS12_381_G1_Element : Kind_Base
+  | K_DefaultUniBLS12_381_G2_Element :
+      |-*_uni DefaultUniBLS12_381_G2_Element : Kind_Base
+  | K_DefaultUniBLS12_381_MlResult :
+      |-*_uni DefaultUniBLS12_381_MlResult : Kind_Base
+  | K_DefaultUniApply k k' t t':
+      |-*_uni t : (Kind_Arrow k k') ->
+      |-*_uni t' : k ->
+      |-*_uni (DefaultUniApply t t') : k'
+  | K_DefaultUniProtoPair :
+      |-*_uni DefaultUniProtoPair : (Kind_Arrow Kind_Base (Kind_Arrow Kind_Base Kind_Base))
+  | K_DefaultUniProtoList :
+      |-*_uni DefaultUniProtoList : (Kind_Arrow Kind_Base Kind_Base)
+  where "'|-*_uni' T ':' K" := (has_kind_uni T K)
+.
+
+
+(* Example ill-kinded:
+nil |-* TyApp (Lam bX Kind_Base "bX") (Lam bY Kind_Base "bY")
+
+So then: nil |-* (Lam bY Kind_Base "bY") : K1a -> K1b
+(bY, Kind_Base) |-* "bY" : Kind_Base = K1b
+also K1a = K1b = Kind_Base
+Hence K1 := Kind_Base -> Kind_Base
+
+lam bX Kind_Base "bX" : (KB -> KB) -> K2 ?
+No, because it is KB -> KB in total.
+No way to unify (KB -> KB) -> K2 with KB -> KB
+
+*)
+
+(** Kinding of types *)
+Reserved Notation "Δ '|-*' T ':' K" (at level 40, T at level 0, K at level 0).
+Inductive has_kind : list (binderName * kind) -> ty -> kind -> Set :=
+  | K_Var : forall Δ X K,
+      lookup X Δ = Some K ->
+      Δ |-* (Ty_Var X) : K
+  | K_Fun : forall Δ T1 T2,
+      Δ |-* T1 : Kind_Base ->
+      Δ |-* T2 : Kind_Base ->
+      Δ |-* (Ty_Fun T1 T2) : Kind_Base
+  | K_IFix  : forall Δ F T K,
+      Δ |-* T : K ->
+      Δ |-* F : (Kind_Arrow (Kind_Arrow K Kind_Base) (Kind_Arrow K Kind_Base)) ->
+      Δ |-* (Ty_IFix F T) : Kind_Base
+  | K_Forall : forall Δ X K T,
+      ((X, K) :: Δ) |-* T : Kind_Base ->
+      Δ |-* (Ty_Forall X K T) : Kind_Base
+  | K_Builtin : forall Δ T,
+      |-*_uni T : Kind_Base ->
+      Δ |-* (Ty_Builtin T) : Kind_Base (* DefaultUni built in types must be fully applied with K_DefaultUniApply *)
+  | K_Lam : forall Δ X K1 T K2,
+      ((X, K1) :: Δ) |-* T : K2 ->
+      Δ |-* (Ty_Lam X K1 T) : (Kind_Arrow K1 K2)
+  | K_App : forall Δ T1 T2 K1 K2,
+      Δ |-* T1 : (Kind_Arrow K1 K2) ->
+      Δ |-* T2 : K1 ->
+      Δ |-* (Ty_App T1 T2) : K2
+where "Δ '|-*' T ':' K" := (has_kind Δ T K).
